As mentioned in the last Skype call, the [Term] datatype of L1g, L1_5, L2 and L3 now containg a constructor [TWrong], and compiling no longer returns option or exception.  THIS WILL BREAK SOMETHING IN L4, which I haven't fixed.
I made lots of other changes.  The only other change I think may be
observable to other levels of the compiler is that wcbvEval of L3
(both the relation and the function versions) is slightly more
liberal.  This change should not be observable for terms that come
from Coq.  (This is a time dependent claim, as Coq might change, and
the arbitrary internal representation that template-coq represents may
change.)

Updating before this commit, I had a good deal of frustration fixing
conflicts introduced by Matthieu (and a minor one by Abhishek).  Every
file in L3 had a conflict.  I realize Matthieu changed template-coq,
which naturally propogates through the whole compiler, but making the
changes for myself would leave me in better mood than fixing conflicts
and merges that didn't work in many files.

In future PLEASE DON'T CHANGE MY FILES WITHOUT FIRST EMAILING ME ABOUT
IT!!!.  Remember I am currently responsible for languages L1g, L1_5,
L2 and L3, which is a lot of files for conflicts.

theories/L1_5_box/compile.v
@@ -17,12 +17,12 @@ Local Open Scope bool.
 Local Open Scope list.
 Set Implicit Arguments.
 
-Definition L1Term := L1g.compile.Term.
-Definition L1Terms := L1g.compile.Terms.
-Definition L1Defs := L1g.compile.Defs.
-Definition L1EC := L1g.compile.envClass.
-Definition L1Env := L1g.compile.environ.
-Definition L1Pgm := L1g.compile.Program.
+Definition L1gTerm := L1g.compile.Term.
+Definition L1gTerms := L1g.compile.Terms.
+Definition L1gDefs := L1g.compile.Defs.
+Definition L1gEC := envClass L1gTerm.
+Definition L1gEnv := environ L1gTerm.
+Definition L1gPgm := Program L1gTerm.
 
 
 Inductive Term : Type :=
@@ -36,11 +36,14 @@ Inductive Term : Type :=
                Term (* dfn *) -> Term (* type *) -> Term (* body *) -> Term
 | TApp       : Term -> Term (* first arg must exist *) -> Terms -> Term
 | TConst     : string -> Term
+| TAx        : Term
 | TInd       : inductive -> Term
-| TConstruct : inductive -> nat -> Term
+| TConstruct : inductive -> nat (* index in datatype *) ->
+               nat (* arity *) -> Term
 | TCase      : (inductive * nat * list nat) (* # of parameters, args per branch *) ->
                Term (* type info *) -> Term -> Terms -> Term
 | TFix       : Defs -> nat -> Term
+| TWrong     : Term
 with Terms : Type :=
 | tnil : Terms
 | tcons : Term -> Terms -> Terms
@@ -53,9 +56,6 @@ Scheme Trm_ind' := Induction for Term Sort Prop
   with Defs_ind' := Induction for Defs Sort Prop.
 Combined Scheme TrmTrmsDefs_ind from Trm_ind', Trms_ind', Defs_ind'.
 Combined Scheme TrmTrms_ind from Trm_ind', Trms_ind'.
-Scheme Trm_ind2 := Induction for Term Sort Type
-  with Trms_ind2 := Induction for Terms Sort Type
-  with Defs_ind2 := Induction for Defs Sort Type.
 Notation prop := (TSort SProp).
 Notation set_ := (TSort SSet).
 Notation type_ := (TSort SType).
@@ -127,79 +127,71 @@ Fixpoint applyBranchToProof (br:Term) :=
     | x => x
   end.
 
-Function L1Term_Term (t:L1Term) : Term :=
+Function L1gTerm_Term (t:L1gTerm) : Term :=
   match t with
     | L1g.compile.TRel n => TRel n
     | L1g.compile.TSort srt => TSort srt
     | L1g.compile.TCast _ _ (L1g.compile.TCast _ _ (L1g.compile.TSort SProp)) =>
       TProof
     | L1g.compile.TCast tm ck ty =>
-      TCast (L1Term_Term ty) ck (L1Term_Term tm)
+      TCast (L1gTerm_Term ty) ck (L1gTerm_Term tm)
     | L1g.compile.TProd nm ty bod =>
-      TProd nm (L1Term_Term ty) (L1Term_Term bod)
+      TProd nm (L1gTerm_Term ty) (L1gTerm_Term bod)
     | L1g.compile.TLambda nm ty bod =>
-      TLambda nm (L1Term_Term ty) (L1Term_Term bod)
+      TLambda nm (L1gTerm_Term ty) (L1gTerm_Term bod)
     | L1g.compile.TLetIn nm dfn ty bod =>
-      TLetIn nm (L1Term_Term dfn) (L1Term_Term ty) (L1Term_Term bod)
+      TLetIn nm (L1gTerm_Term dfn) (L1gTerm_Term ty) (L1gTerm_Term bod)
     | L1g.compile.TApp fn arg args =>
-      TApp (L1Term_Term fn) (L1Term_Term arg) (L1Terms_Terms args)
+      TApp (L1gTerm_Term fn) (L1gTerm_Term arg) (L1gTerms_Terms args)
     | L1g.compile.TConst pth => TConst pth
+    | L1g.compile.TAx => TAx
     | L1g.compile.TInd ind => TInd ind
-    | L1g.compile.TConstruct ind m => TConstruct ind m
+    | L1g.compile.TConstruct ind m arty => TConstruct ind m arty
     | L1g.compile.TCase m ty mch brs =>
-      match L1Term_Term mch, L1Terms_Terms brs with
+      match L1gTerm_Term mch, L1gTerms_Terms brs with
         | TProof, tunit br => applyBranchToProof br
-        | Mch, Brs => TCase m (L1Term_Term ty) Mch Brs
+        | Mch, Brs => TCase m (L1gTerm_Term ty) Mch Brs
       end
-    | L1g.compile.TFix defs m => TFix (L1Defs_Defs defs) m
+    | L1g.compile.TFix defs m => TFix (L1gDefs_Defs defs) m
+    | L1g.compile.TWrong _ => TWrong
   end
-with L1Terms_Terms (ts:L1Terms) : Terms :=
+with L1gTerms_Terms (ts:L1gTerms) : Terms :=
        match ts with
          | L1g.compile.tnil => tnil
-         | L1g.compile.tcons u us => tcons (L1Term_Term u) (L1Terms_Terms us)
+         | L1g.compile.tcons u us => tcons (L1gTerm_Term u) (L1gTerms_Terms us)
        end
-with L1Defs_Defs (ds:L1Defs) : Defs :=
+with L1gDefs_Defs (ds:L1gDefs) : Defs :=
        match ds with
          | L1g.compile.dnil => dnil
          | L1g.compile.dcons nm ty tm m ds =>
-           dcons nm (L1Term_Term ty) (L1Term_Term tm) m (L1Defs_Defs ds)
+           dcons nm (L1gTerm_Term ty) (L1gTerm_Term tm) m (L1gDefs_Defs ds)
        end.
 (****
-Functional Scheme L1Term_Term_ind' := Induction for L1Term_Term Sort Prop
+Functional Scheme L1gTerm_Term_ind' := Induction for L1gTerm_Term Sort Prop
 with terms_Terms_ind' := Induction for terms_Terms Sort Prop
 with wcbvDEvals_ind' := Induction for defs_Defs Sort Prop.
-Combined Scheme L1Term_TermEvalsDEvals_ind
-         from L1Term_Term_ind', terms_Terms_ind', wcbvDEvals_ind'.
+Combined Scheme L1gTerm_TermEvalsDEvals_ind
+         from L1gTerm_Term_ind', terms_Terms_ind', wcbvDEvals_ind'.
 ***)
 
 (** environments and programs **)
-Definition envClass := AstCommon.envClass Term.
-Definition environ := AstCommon.environ Term.
-Definition Program := AstCommon.Program Term.
-
-Function L1EC_EC (ec:L1EC) : envClass :=
+Function L1gEC_EC (ec:L1gEC) : envClass Term :=
   match ec with
-    | ecTrm t => ecTrm (L1Term_Term t)
+    | ecTrm t => ecTrm (L1gTerm_Term t)
     | ecTyp _ n itp => ecTyp Term n itp
   end.
 
-Definition L1Env_Env: L1Env -> environ :=
-  List.map (fun (nmec: string * L1EC) => (fst nmec, L1EC_EC (snd nmec))).
+Definition L1gEnv_Env: L1gEnv -> environ Term :=
+  List.map (fun (nmec: string * L1gEC) => (fst nmec, L1gEC_EC (snd nmec))).
 
-Definition L1Pgm_Program (p:L1Pgm) : Program :=
-  {| env:= L1Env_Env (env p);
-     main:= L1Term_Term (main p) |}.
+Definition L1gPgm_Program (p:L1gPgm) : Program Term:=
+  {| env:= L1gEnv_Env (env p);
+     main:= L1gTerm_Term (main p) |}.
 
 
 (*** from L1 to L1_5 ***)
-Definition program_Program (p:program) : exception Program :=
-  match L1g.compile.program_Program p (Ret nil) with
-    | Exc s => raise s
-    | Ret q => Ret (L1Pgm_Program q)
-  end.
-Definition term_Term (t:term) : exception Term :=
-  match L1g.compile.term_Term t with
-    | Exc s => raise s
-    | Ret q => Ret (L1Term_Term q)
-  end.
+Definition program_Program (p:program) : Program Term :=
+  L1gPgm_Program (L1g.compile.program_Program p).
 
+Definition term_Term (e:AstCommon.environ L1gTerm) (t:term) : Term :=
+  L1gTerm_Term (L1g.compile.term_Term e t).
