theories/L3_flattenedApp/unaryApplications.v
@@ -1,12 +1,9 @@
 (******)
 Add LoadPath "../common" as Common.
-Add LoadPath "../L1_MalechaQuoted" as L1.
 Add LoadPath "../L1_5_box" as L1_5.
 Add LoadPath "../L2_typeStripped" as L2.
 Add LoadPath "../L3_flattenedApp" as L3.
 (******)
-
-Require L2.compile.
 
 Require Import Coq.Lists.List.
 Require Import Coq.Strings.String.
@@ -14,6 +11,7 @@ Require Import Coq.Strings.Ascii.
 Require Import Coq.Arith.Compare_dec.
 Require Import Coq.Arith.Minus.
 Require Import Coq.Logic.JMeq.
+Require Import Omega.
 Require Import L2.L2.
 Require Import L3.term.
 Require Import L3.program.
@@ -30,168 +28,272 @@ Set Implicit Arguments.
 Definition L2Term := L2.compile.Term.
 Definition L2Terms := L2.compile.Terms.
 Definition L2Defs := L2.compile.Defs.
+Definition L2Environ := AstCommon.environ L2.compile.Term.
 
-
-Lemma strip_Lam_invrt:
-  forall p nm bod tt,
-        strip p (L2.compile.TLambda nm bod) = Ret tt ->
-        exists sbod, strip p bod = Ret sbod /\ tt = TLambda nm sbod.
-Proof.
-  induction tt; simpl; intros. 
-  - change ((match strip p bod with
-              | Ret sbod => Ret (TLambda nm sbod)
-              | Exc s => Exc s end) = Ret (TRel n)) in H.
-    destruct (strip p bod); discriminate.
-  - change ((match strip p bod with
-              | Ret sbod => Ret (TLambda nm sbod)
-              | Exc s => Exc s end) = Ret (TSort s)) in H.
-    destruct (strip p bod); discriminate.
-  - change ((match strip p bod with
-              | Ret sbod => Ret (TLambda nm sbod)
-              | Exc s => Exc s end) = Ret TProof) in H.
-     destruct (strip p bod); discriminate.
-  - change ((match strip p bod with
-              | Ret sbod => Ret (TLambda nm sbod)
-              | Exc s => Exc s end) = Ret (TProd n tt)) in H.
-    destruct (strip p bod); discriminate.
-  - change ((match strip p bod with
-              | Ret sbod => Ret (TLambda nm sbod)
-              | Exc s => Exc s end) = Ret (TLambda n tt)) in H.
-    destruct (strip p bod).
-    + discriminate. 
-    + myInjection H. exists tt. intuition.
-  - change ((match strip p bod with
-              | Ret sbod => Ret (TLambda nm sbod)
-              | Exc s => Exc s end) = Ret (TLetIn n tt1 tt2)) in H.
-    destruct (strip p bod); discriminate.
-  - change ((match strip p bod with
-              | Ret sbod => Ret (TLambda nm sbod)
-              | Exc s => Exc s end) = Ret (TApp tt1 tt2)) in H.
-    destruct (strip p bod); discriminate.
-  - change ((match strip p bod with
-              | Ret sbod => Ret (TLambda nm sbod)
-              | Exc s => Exc s end) = Ret (TConst s)) in H.
-    destruct (strip p bod); discriminate.
-  - change ((match strip p bod with
-              | Ret sbod => Ret (TLambda nm sbod)
-              | Exc s => Exc s end) = Ret TAx) in H.
-    destruct (strip p bod); discriminate.    
-  - change ((match strip p bod with
-              | Ret sbod => Ret (TLambda nm sbod)
-              | Exc s => Exc s end) = Ret (TInd i)) in H.
-    destruct (strip p bod); discriminate.
-  - change ((match strip p bod with
-              | Ret sbod => Ret (TLambda nm sbod)
-              | Exc s => Exc s end) = Ret (TConstruct i n t)) in H.
-    destruct (strip p bod); discriminate.
-  - change ((match strip p bod with
-              | Ret sbod => Ret (TLambda nm sbod)
-              | Exc s => Exc s end) = Ret (TCase p0 tt t)) in H.
-    destruct (strip p bod); discriminate.
-  - change ((match strip p bod with
-              | Ret sbod => Ret (TLambda nm sbod)
-              | Exc s => Exc s end) = Ret (TFix d n)) in H.
-    destruct (strip p bod); discriminate.
+Lemma TApp_hom:
+  forall fn arg args,
+    strip (L2.compile.TApp fn arg args) =
+    let sarg := strip arg in
+      let sargs := strips args in
+      match fn with 
+        | L2.compile.TConstruct i n arty =>
+          etaExp_cnstr i n arty (tcons sarg sargs)
+        | x => mkApp (strip x) (tcons sarg sargs)
+       end.
+  induction fn; cbn; intros; try reflexivity.
+Qed.
+    
+Lemma TFix_hom:
+  forall defs n,
+    strip (L2.compile.TFix defs n) = TFix (stripDs defs) n.
+reflexivity.
 Qed.
 
-Lemma strip_Prod_invrt:
-  forall p nm bod tt,
-        strip p (L2.compile.TProd nm bod) = Ret tt ->
-        exists sbod, strip p bod = Ret sbod /\ tt = TProd nm sbod.
-Proof.
-  induction tt; simpl; intros. 
-  - change ((match strip p bod with
-              | Ret sbod => Ret (TProd nm sbod)
-              | Exc s => Exc s end) = Ret (TRel n)) in H.
-    destruct (strip p bod); discriminate.
-  - change ((match strip p bod with
-              | Ret sbod => Ret (TProd nm sbod)
-              | Exc s => Exc s end) = Ret (TSort s)) in H.
-    destruct (strip p bod); discriminate.
-  - change ((match strip p bod with
-              | Ret sbod => Ret (TProd nm sbod)
-              | Exc s => Exc s end) = Ret TProof) in H.
-    destruct (strip p bod); discriminate.
-  - change ((match strip p bod with
-              | Ret sbod => Ret (TProd nm sbod)
-              | Exc s => Exc s end) = Ret (TProd n tt)) in H.
-    destruct (strip p bod). 
-    + discriminate.
-    + myInjection H. exists tt. intuition.
-  - change ((match strip p bod with
-              | Ret sbod => Ret (TProd nm sbod)
-              | Exc s => Exc s end) = Ret (TLambda n tt)) in H.
-    destruct (strip p bod); discriminate.
-  - change ((match strip p bod with
-              | Ret sbod => Ret (TProd nm sbod)
-              | Exc s => Exc s end) = Ret (TLetIn n tt1 tt2)) in H.
-    destruct (strip p bod); discriminate.
-  - change ((match strip p bod with
-              | Ret sbod => Ret (TProd nm sbod)
-              | Exc s => Exc s end) = Ret (TApp tt1 tt2)) in H.
-    destruct (strip p bod); discriminate.
-  - change ((match strip p bod with
-              | Ret sbod => Ret (TProd nm sbod)
-              | Exc s => Exc s end) = Ret (TConst s)) in H.
-    destruct (strip p bod); discriminate.
-  - change ((match strip p bod with
-              | Ret sbod => Ret (TProd nm sbod)
-              | Exc s => Exc s end) = Ret TAx) in H.
-    destruct (strip p bod); discriminate.
-  - change ((match strip p bod with
-              | Ret sbod => Ret (TProd nm sbod)
-              | Exc s => Exc s end) = Ret (TInd i)) in H.
-    destruct (strip p bod); discriminate.
-  - change ((match strip p bod with
-              | Ret sbod => Ret (TProd nm sbod)
-              | Exc s => Exc s end) = Ret (TConstruct i n t)) in H.
-    destruct (strip p bod); discriminate.
-  - change ((match strip p bod with
-              | Ret sbod => Ret (TProd nm sbod)
-              | Exc s => Exc s end) = Ret (TCase p0 tt t)) in H.
-    destruct (strip p bod); discriminate.
-  - change ((match strip p bod with
-              | Ret sbod => Ret (TProd nm sbod)
-              | Exc s => Exc s end) = Ret (TFix d n)) in H.
-    destruct (strip p bod); discriminate.
+Lemma TProd_hom:
+  forall nm bod,
+    strip (L2.compile.TProd nm bod) = TProd nm (strip bod).
+reflexivity.
 Qed.
 
-Lemma strip_Construct_invrt:
-  forall p i r tt,
-        strip p (L2.compile.TConstruct i r) = Ret tt ->
-        etaExp_cnstr p i r tnil = Ret tt.
+Lemma TLambda_hom:
+  forall nm bod,
+    strip (L2.compile.TLambda nm bod)  = TLambda nm (strip bod).
 Proof.
-  induction tt; unfold strip; simpl; intros; try assumption.
-Qed.
- 
-Lemma strip_Ind_invrt:
-  forall p i tt,
-        strip p (L2.compile.TInd i) = Ret tt -> tt = (TInd i).
-Proof.
-  induction tt;  simpl; intros; try discriminate.
-  myInjection H. reflexivity.
+  reflexivity.
 Qed.
 
-(********
+Lemma TLetIn_hom:
+  forall nm dfn bod,
+    strip (L2.compile.TLetIn nm dfn bod) =
+    TLetIn nm (strip dfn) (strip bod).
+reflexivity.
+Qed.
+
+Lemma TCase_hom:
+  forall n mch brs,
+    strip (L2.compile.TCase n mch brs) =
+    TCase n (strip mch) (strips brs).
+reflexivity.
+Qed.
+
+Lemma TConstruct_hom:
+  forall i n arty,
+    strip (L2.compile.TConstruct i n arty) = etaExp_cnstr i n arty tnil.
+Proof.
+  reflexivity.  
+Qed.
+
+Lemma TInd_hom:
+  forall i,
+        strip (L2.compile.TInd i) = (TInd i).
+Proof.
+  reflexivity.
+Qed.
+
+Lemma Lookup_hom:
+  forall (p:environ L2Term) (s:string) ec,
+    Lookup s p ec -> Lookup s (stripEnv p) (stripEC ec).
+Proof.
+  induction 1; destruct t.
+  - cbn. apply LHit.
+  - cbn. apply LHit.
+  - cbn. apply LMiss; assumption. 
+  - cbn. apply LMiss; assumption. 
+Qed.
+
+Lemma dlength_hom:
+  forall ds, L2.term.dlength ds = dlength (stripDs ds).
+induction ds. intuition. cbn. rewrite IHds. reflexivity.
+Qed.
+
+Lemma tcons_hom:
+  forall t ts, strips (L2.compile.tcons t ts) = tcons (strip t) (strips ts).
+reflexivity.
+Qed.
+
+Lemma tappend_hom:
+  forall ts us,
+    strips (L2.term.tappend ts us) = tappend (strips ts) (strips us).
+induction ts; intros us; simpl. reflexivity.
+rewrite IHts. reflexivity.
+Qed.
+
+
+Lemma mkApp_hom:
+forall fn args,
+  strip (L2.term.mkApp fn args) = mkApp (strip fn) (strips args).
+Proof.
+  induction fn; induction args; cbn; try reflexivity.
+  - rewrite L2.term.tappend_tnil. reflexivity.
+  - rewrite tappend_hom. rewrite tcons_hom.
+    admit.
+Admitted.
+
+Lemma instantiate_hom:
+    (forall bod arg n, strip (L2.term.instantiate arg n bod) =
+                   instantiate (strip arg) n (strip bod)) /\
+    (forall bods arg n, strips (L2.term.instantiates arg n bods) =
+                    instantiates (strip arg) n (strips bods)) /\
+    (forall ds arg n, stripDs (L2.term.instantiateDefs arg n ds) =
+                      instantiateDefs (strip arg) n (stripDs ds)).
+Proof.
+  apply L2.compile.TrmTrmsDefs_ind; intros; try (simpl; reflexivity).
+  - simpl. destruct (lt_eq_lt_dec n n0); cbn.
+    + destruct s.
+      * rewrite (proj1 (nat_compare_gt n0 n)); try omega. reflexivity.
+      * subst. rewrite (proj2 (nat_compare_eq_iff _ _)); trivial.
+        rewrite mkApp_tnil_ident. reflexivity.
+    + rewrite (proj1 (nat_compare_lt n0 n)); trivial.
+  - change (strip (L2.term.instantiate arg n t) =
+            (instantiate (strip arg) n (strip t))).
+    rewrite H. reflexivity.
+  - change (TProd n (strip (L2.term.instantiate arg (S n0) t)) =
+            (TProd n (instantiate (strip arg) (S n0) (strip t)))).
+    rewrite H. reflexivity.
+  - change (TLambda n (strip (L2.term.instantiate arg (S n0) t)) =
+            (TLambda n (instantiate (strip arg) (S n0) (strip t)))).
+    rewrite H. reflexivity.
+  - change (TLetIn n (strip (L2.term.instantiate arg n0 t))
+                   (strip (L2.term.instantiate arg (S n0) t0)) =
+            (TLetIn n (instantiate (strip arg) n0 (strip t))
+                    (instantiate (strip arg) (S n0) (strip t0)))).
+    rewrite H. rewrite H0. reflexivity.
+  - change (strip (L2.term.mkApp
+                     (L2.term.instantiate arg n t)
+                     (L2.compile.tcons (L2.term.instantiate arg n t0)
+                                       (L2.term.instantiates arg n t1))) =
+            instantiate (strip arg) n (strip (L2.compile.TApp t t0 t1))).
+    admit.
+  (*************
+  rewrite TApp_hom. destruct t; cbn.
+  change
+    (strip (L2.term.mkApp (L2.term.instantiate arg n t)
+                          (L2.compile.tcons (L2.term.instantiate arg n t0)
+                                         (L2.term.instantiates arg n t1))) =
+     (mkApp (instantiate (strip arg) n (strip t))
+            (tcons (instantiate (strip arg) n (strip t0))
+                   (instantiates (strip arg) n (strips t1))))).
+  rewrite <- H. rewrite <- H0. rewrite <- H1. 
+  rewrite mkApp_hom. rewrite tcons_hom. reflexivity.
+   *********************)
+  - cbn. induction n0; try reflexivity. cbn. admit.
+    
+  - change (TCase p (strip (L2.term.instantiate arg n t))
+                    (strips (L2.term.instantiates arg n t0)) =
+              (TCase p (instantiate (strip arg) n (strip t))
+                     (instantiates (strip arg) n (strips t0)))).
+    rewrite H0. rewrite H. reflexivity.
+  - change (TFix (stripDs (L2.term.instantiateDefs
+                             arg (n0 + L2.term.dlength d) d)) n =
+            (TFix (instantiateDefs (strip arg)
+                                   (n0 + dlength (stripDs d)) (stripDs d)) n)).
+    rewrite H. rewrite dlength_hom. reflexivity.
+  - change (tcons (strip (L2.term.instantiate arg n t))
+                  (strips (L2.term.instantiates arg n t0)) =
+            tcons (instantiate (strip arg) n (strip t))
+                  (instantiates (strip arg) n (strips t0))).
+    rewrite H. rewrite H0. reflexivity.
+  - change (dcons n (strip (L2.term.instantiate arg n1 t)) n0
+                  (stripDs (L2.term.instantiateDefs arg n1 d)) =
+            dcons n (instantiate (strip arg) n1 (strip t)) n0
+                  (instantiateDefs (strip arg) n1 (stripDs d))).
+    rewrite H0. rewrite H. reflexivity.
+Admitted.
+
+(*****
+Lemma whBetaStep_hom:
+  forall bod arg args,
+    strip (L2.term.whBetaStep bod arg args) =
+    whBetaStep (strip bod) (strip arg) (strips args).
+intros bod arg args.
+unfold L1_5.term.whBetaStep, whBetaStep.
+rewrite mkApp_hom. rewrite <- (proj1 instantiate_hom). reflexivity.
+Qed.
+ *****)
+
+Lemma whBetaStep_hom:
+  forall bod arg args,
+    strip (L2.term.whBetaStep bod arg args) =
+    mkApp (whBetaStep (strip bod) (strip arg)) (strips args).
+Admitted.
+(*******
+Proof.
+  induction args; cbn; intros.
+  - unfold L2.term.whBetaStep, whBetaStep.
+    rewrite L2.term.mkApp_tnil_ident. apply (proj1 instantiate_hom).
+  - unfold L2.term.whBetaStep, whBetaStep.
+    unfold L2.term.whBetaStep, whBetaStep in IHargs.
+    rewrite <- (proj1 instantiate_hom) in IHargs.
+    
+
+ rewrite <- (proj1 instantiate_hom). 
+   unfold mkApp.
+    destruct (L2.term.instantiate arg 0 bod); cbn.
+******)
+
+(*********************
 Lemma WcbvEval_hom:
-  forall (p:AstCommon.environ L2Term) L3p, stripEnv p = Ret L3p ->
+  forall (p:L2Env), 
   (forall t t': L2Term, L2.wcbvEval.WcbvEval p t t' ->
-    forall L3t, strip p t = Ret L3t ->
-    forall L3t', strip p t' = Ret L3t' ->
-        WcbvEval L3p L3t L3t') /\
+                        L3.wcbvEval.WcbvEval (L3.compile.stripEnv p)
+                                             (L3.compile.strip t)
+                                             (L3.compile.strip t')) /\
   (forall ts ts', L2.wcbvEval.WcbvEvals p ts ts' ->
-    forall L3ts, strips p ts = Ret L3ts ->
-    forall L3ts', strips p ts' = Ret L3ts' ->
-                  WcbvEvals L3p L3ts L3ts') /\
-  (forall ds ds', L2.wcbvEval.WcbvDEvals p ds ds' -> True).
-(*************
-    forall L3ds, stripDs p ds = Ret L3ds ->
-    forall L3ds', stripDs p ds' = Ret L3ds' ->
-                     WcbvDEvals L3p L3ds L3ds').
-****************)
+                  L3.wcbvEval.WcbvEvals (L3.compile.stripEnv p)
+                                        (L3.compile.strips ts)
+                                        (L3.compile.strips ts')).
 Proof.
-  intros p L3p hp.
-  apply L2.wcbvEval.WcbvEvalEvals_ind; cbn; intros; try reflexivity.
+  intros p.
+  apply L2.wcbvEval.WcbvEvalEvals_ind; cbn; intros; try reflexivity;
+  try intuition; try (rewrite <- H; rewrite <- H0; constructor).
+  - induction arty.
+    + constructor. constructor.
+    + cbn. rewrite mkEta_under_Lambda. constructor. 
+  - econstructor. unfold LookupDfn in l. unfold LookupDfn. apply (Lookup_hom l).
+    assumption.
+  - destruct (L2.term.isLambda_dec fn).
+    + destruct i as [x0 [x1 j0]]. rewrite j0. induction args; cbn.
+      * repeat econstructor. inversion_Clear H0. eassumption.
+        rewrite whBetaStep_hom in H1.
+        
+exact H1.
+    
+
+
+    
+  - destruct (L2.term.isLambda_dec fn).
+    + destruct i as [x0 [x1 j0]]. rewrite j0. cbn; destruct a1; cbn.
+      assert (k:= TApp_hom (L2.compile.TLambda x0 x1)). cbn in k.
+
+
+    ; destruct args; cbn.
+    + econstructor. inversion w. 
+    
+  - unfold LookupDfn in l. rewrite (Lookup_lookup l).
+    econstructor. unfold LookupDfn. apply Lookup_hom.
+    inversion_Clear l.
+
+    
+    inversion_Clear l. cbn. rewrite string_eq_bool_rfl.
+    unfold program.ecAx. unfold AstCommon.ecAx. cbn.
+    constructor.
+    Check (stripEnv_not_LookupAx p).
+    Check (Lookup_hom l). destruct (lookup nm p).
+    + constructor. 
+    + destruct e.
+      * unfold AstCommon.LookupDfn.inversion l.
+      * eapply wConst. unfold AstCommon.LookupDfn. Print AstCommon.ecAx.
+        unfold AstCommon.ecAx in l.
+        change ((@AstCommon.Lookup Term) nm p (AstCommon.ecAx Term)) in l.
+        Check (Lookup_hom l).
+
+        rewrite <- H. eapply wConst.
+        unfold AstCommon.LookupDfn.
+        Check Lookup_hom. apply Lookup_hom.
+      unfold LookupAx in l.
+
+    rewrite <- H0. rewrite <- H1.
+    
   - myInjection H. myInjection H0. constructor.
   - case_eq (strip p bod); intros x hx; rewrite hx in *.
     + discriminate.
@@ -206,26 +308,29 @@ Proof.
 *******)
 
 
-      
 (**** L2 and L3 agree on cbv evaluation  ****
 Lemma wndEval_types_irrelevant:
-  forall p pp, stripEnv p = Some pp -> 
-    (forall t s, L2.wcbvEval.WcbvEval p t s ->
-     forall tt, strip p t = Some tt -> 
-     forall ss, strip p s = Some ss ->
-          WcbvEval pp tt ss) /\
-    (forall ts ss, L2.wcbvEval.WcbvEvals p ts ss ->
-     forall tss, strips p ts = Some tss -> 
-     forall sss, strips p ss = Some sss ->
-          WcbvEvals pp tss sss).
+  forall (p:L2Environ),
+    (forall (t s:L2Term),
+       L2.wcbvEval.WcbvEval p t s ->
+       WcbvEval (stripEnv p) (strip p t) (strip p s))  /\
+    (forall ts ss,
+       L2.wcbvEval.WcbvEvals p ts ss ->
+       WcbvEvals (stripEnv p) (strips p ts) (strips p ss)).
 Proof.
-  intros p pp h. apply L2.wcbvEval.WcbvEvalEvals_ind; simpl; intros.
-  - destruct (strip_Lam_invrt _ _ _ H) as [x [j1x j2x]].
-    destruct (strip_Lam_invrt _ _ _ H0) as [y [j1y j2y]].
-    subst. rewrite j1x in j1y. myInjection j1y. constructor.
-  - destruct (strip_Prod_invrt _ _ _ H) as [x [j1x j2x]].
-    destruct (strip_Prod_invrt _ _ _ H0) as [y [j1y j2y]].
-    subst. rewrite j1x in j1y. myInjection j1y. constructor.
+  intros p.
+  apply L2.wcbvEval.WcbvEvalEvals_ind; intros; try reflexivity;
+  try (solve[constructor; trivial]); try assumption.
+  - admit. (** rewrite TConstruct_hom.  cbn. **)
+  - unfold LookupAx in l. cbn. assert (j:= Lookup_lookup l). 
+    Check j. Check (lookup nm p).
+    destruct (lookup nm p).
+    + destruct e. refine (wConst _ _). unfold AstCommon.LookupDfn.
+    rewrite j.
+
+    
+  - rewrite TFix_hom. rewrite TFix_hom. 
+    
   - change (strip p t = Some tt) in H0. eapply H; assumption.
   - unfold strip in H. unfold strip in H0. rewrite H in H0.
     myInjection H0. clear H0. unfold etaExp_cnstr in H.
